code/curve25519/Hacl.Bignum.Fdifference.fst
@@ -16,21 +16,31 @@ let gte_limbs_c h (a:felem) h' (b:felem) (l:nat{l <= len}) : GTot Type0 =
   live h a /\ live h' b /\ gte_limbs (as_seq h a) (as_seq h' b) l
 
 
-[@"c_inline"]
-val fdifference_:
+[@"substitute"]
+inline_for_extraction val fdifference_:
   a:felem ->
   b:felem{disjoint a b} ->
   i:ctr{U32.v i <= len} ->
   Stack unit
-    (requires (fun h -> gte_limbs_c h a h b (U32.v i)))
+    (requires (fun h -> len = 5 /\ gte_limbs_c h a h b (U32.v i)))
     (ensures (fun h0 _ h1 -> gte_limbs_c h0 a h0 b (U32.v i) /\ live h1 a /\ modifies_1 a h0 h1
       /\ as_seq h1 a == fdifference_spec (as_seq h0 a) (as_seq h0 b) (U32.v i)))
-[@"c_inline"]
-let rec fdifference_ a b i =
-  if U32.(i =^ 0ul) then ()
-  else (
-    let i = U32.(i -^ 1ul) in
-    let ai = a.(i) in let bi = b.(i) in
-    a.(i) <- bi -^ ai;
-    fdifference_ a b i
-  )
+[@"substitute"]
+inline_for_extraction let rec fdifference_ a b i =
+    let a0 = a.(0ul) in 
+    let b0 = b.(0ul) in
+    let a1 = a.(1ul) in 
+    let b1 = b.(1ul) in
+    let a2 = a.(2ul) in 
+    let b2 = b.(2ul) in
+    let a3 = a.(3ul) in 
+    let b3 = b.(3ul) in
+    let a4 = a.(4ul) in 
+    let b4 = b.(4ul) in
+
+    a.(0ul) <- b0 -^ a0;
+    a.(1ul) <- b1 -^ a1;
+    a.(2ul) <- b2 -^ a2;
+    a.(3ul) <- b3 -^ a3;
+    a.(4ul) <- b4 -^ a4
+
