code/curve25519/Hacl.Bignum.Crecip.fst
@@ -24,6 +24,7 @@ private let lemma_5413_is_55 (s:seqelem{red_5413 s}) : Lemma (Hacl.Spec.EC.AddAn
 
 #set-options "--initial_fuel 0 --max_fuel 0 --z3rlimit 20"
 
+[@"substitute"]
 inline_for_extraction private val fmul:
   output:felem ->
   a:felem ->
@@ -39,6 +40,7 @@ inline_for_extraction private val fmul:
       /\ eval h1 output % prime = (eval h0 a * eval h0 b) % prime
       /\ as_seq h1 output == Hacl.Spec.Bignum.fmul_tot (as_seq h0 a) (as_seq h0 b)
       ))
+[@"substitute"]
 inline_for_extraction private let fmul output a b =
   let h = ST.get() in
   lemma_513_is_53 (as_seq h a);
@@ -49,6 +51,7 @@ inline_for_extraction private let fmul output a b =
 
 #reset-options "--initial_fuel 0 --max_fuel 0 --z3rlimit 10"
 
+[@"substitute"]
 inline_for_extraction private val fsquare_times:
   output:felem ->
   input:felem{disjoint output input} ->
@@ -60,12 +63,14 @@ inline_for_extraction private val fsquare_times:
       /\ Hacl.Spec.EC.AddAndDouble.red_513 (as_seq h0 input)
       /\ Hacl.Spec.EC.AddAndDouble.red_513 (as_seq h1 output)
       /\ (as_seq h1 output) == Hacl.Spec.Bignum.Fsquare.fsquare_times_tot (as_seq h0 input) (FStar.UInt32.v count)))
+[@"substitute"]
 inline_for_extraction private let fsquare_times output input count =
   let h = ST.get() in
   lemma_513_is_5413 (as_seq h input);
   fsquare_times output input count
 
 
+[@"substitute"]
 inline_for_extraction private val fsquare_times_inplace:
   output:felem ->
   count:FStar.UInt32.t{FStar.UInt32.v count > 0} ->
@@ -75,6 +80,7 @@ inline_for_extraction private val fsquare_times_inplace:
       /\ Hacl.Spec.EC.AddAndDouble.red_513 (as_seq h0 output)
       /\ Hacl.Spec.EC.AddAndDouble.red_513 (as_seq h1 output)
       /\ (as_seq h1 output) == Hacl.Spec.Bignum.Fsquare.fsquare_times_tot (as_seq h0 output) (FStar.UInt32.v count)))
+[@"substitute"]
 inline_for_extraction private let fsquare_times_inplace output count =
   let h = ST.get() in
   lemma_513_is_5413 (as_seq h output);
@@ -111,6 +117,7 @@ private let lemma_crecip_1_modifies h0 h1 h2 h3 h4 h5 h6 h7 buf =
   lemma_crecip_1_modifies' h0 h7 buf
 
 
+[@"substitute"]
 private inline_for_extraction val crecip_1:
   buf:buffer limb{length buf = 20} ->
   z:felem{disjoint buf z} ->
@@ -128,6 +135,7 @@ private inline_for_extraction val crecip_1:
        /\ ( (as_seq h1 t0, as_seq h1 b, as_seq h1 a)  == crecip_tot_1 (as_seq h0 z)))
   ))
 #reset-options "--initial_fuel 0 --max_fuel 0 --z3rlimit 100"
+[@"substitute"]
 private inline_for_extraction let crecip_1 buf z =
   let a  = Buffer.sub buf 0ul  5ul in
   let t0 = Buffer.sub buf 5ul  5ul in
@@ -175,6 +183,7 @@ private let lemma_crecip_2_modifies h0 h1 h2 h3 h4 h5 h6 h7 h8 buf =
   lemma_crecip_1_modifies' h0 h8 buf
 
 
+[@"substitute"]
 private inline_for_extraction val crecip_2:
   buf:buffer limb{length buf = 20} ->
   Stack unit
@@ -201,6 +210,7 @@ private inline_for_extraction val crecip_2:
        /\ ( (as_seq h1 t0, as_seq h1 b, as_seq h1 a)  == crecip_tot_2 (as_seq h0 t0) (as_seq h0 b) (as_seq h0 a)))
   ))
 #reset-options "--initial_fuel 0 --max_fuel 0 --z3rlimit 200"
+[@"substitute"]
 private inline_for_extraction let crecip_2 buf =
   assert_norm(pow2 32 = 0x100000000);
   let a  = Buffer.sub buf 0ul  5ul in
@@ -260,6 +270,7 @@ private val lemma_crecip_3_modifies: h0:mem -> h1:mem -> h2:mem -> h3:mem -> h4:
 private let lemma_crecip_3_modifies h0 h1 h2 h3 h4 h5 h6 h7 buf out = ()
 
 
+[@"substitute"]
 private inline_for_extraction val crecip_3:
   out:felem ->
   buf:buffer limb{length buf = 20 /\ disjoint out buf} ->
@@ -285,6 +296,7 @@ private inline_for_extraction val crecip_3:
        /\ as_seq h1 out  == crecip_tot_3 (as_seq h0 t0) (as_seq h0 b) (as_seq h0 a))
   ))
 #reset-options "--initial_fuel 0 --max_fuel 0 --z3rlimit 100"
+[@"substitute"]
 private inline_for_extraction let crecip_3 out buf =
   assert_norm(pow2 32 = 0x100000000);
   let a  = Buffer.sub buf 0ul  5ul in
@@ -320,6 +332,7 @@ private inline_for_extraction let crecip_3 out buf =
   lemma_crecip_3_modifies h0 h1 h2 h3 h4 h5 h6 h7 buf out
 
 
+[@"c_inline"]
 val crecip:
   out:felem ->
   z:felem{disjoint out z} ->
@@ -329,6 +342,7 @@ val crecip:
     /\ crecip_pre (as_seq h0 z)
     /\ as_seq h1 out == crecip_tot (as_seq h0 z)
     /\ crecip_pre (as_seq h1 out)))
+[@"c_inline"]
 let crecip out z =
   push_frame();
   let buf = create limb_zero 20ul in
